Polymorphic gmap added

compositionality/Polymorphic_gmap/Polymorphic_gmap.fst
@@ -71,51 +71,125 @@ let merge_idem_b s = ()
 let rc_ind_right_a l a b o1 o2 o2' = ()
 let rc_ind_right_b l a b o1 o2 o2' = ()
 let rc_ind_right_ne l a b o1 o2 o2' = ()
+
 let rc_ind_left_a l a b o1 o2 o1' = ()
 let rc_ind_left_b l a b o1 o2 o1' = ()
 let rc_ind_left_ne l a b o1 o2 o1' = ()
+
 let rc_ind_lca_a l o1 o2 o = ()
 let rc_ind_lca_b l o1 o2 o = ()
 let rc_ind_lca_ne l o1 o2 o = ()
+
 let rc_base o1 o2 t = ()
+
 let rc_inter_base_right_a l a b c o1 o2 ob ol = ()
 let rc_inter_base_right_b l a b c o1 o2 ob ol = ()
 let rc_inter_base_right_ne l a b c o1 o2 ob ol = ()
+
 let rc_inter_base_left_a l a b c o1 o2 ob ol = ()
 let rc_inter_base_left_b l a b c o1 o2 ob ol = ()
 let rc_inter_base_left_ne l a b c o1 o2 ob ol = ()
+
 let rc_inter_right_a l a b c o1 o2 ob ol o = ()
 let rc_inter_right_b l a b c o1 o2 ob ol o = ()
 let rc_inter_right_ne l a b c o1 o2 ob ol o = ()
+
 let rc_inter_left_a l a b c o1 o2 ob ol o = ()
 let rc_inter_left_b l a b c o1 o2 ob ol o = ()
 let rc_inter_left_ne l a b c o1 o2 ob ol o = ()
+
 let rc_inter_lca_a l a b c o1 o2 ol oi = ()
 let rc_inter_lca_b l a b c o1 o2 ol oi = ()
 let rc_inter_lca_ne l a b c o1 o2 ol oi = ()
+
 let one_op_ind_right_a l a b o2 o2' = ()
 let one_op_ind_right_b l a b o2 o2' = ()
 let one_op_ind_right_ne l a b o2 o2' = ()
+
 let one_op_ind_left_a l a b o1 o1' = ()
 let one_op_ind_left_b l a b o1 o1' = ()
 let one_op_ind_left_ne l a b o1 o1' = ()
+
 let one_op_ind_lca_a l o2 o = ()
 let one_op_ind_lca_b l o2 o = ()
 let one_op_ind_lca_ne l o2 o = ()
+
 let one_op_base_a o2 = ()
 let one_op_base_b o2 = ()
+
 let one_op_inter_base_right_a l a b c o2 ob ol = ()
 let one_op_inter_base_right_b l a b c o2 ob ol = ()
 let one_op_inter_base_right_ne l a b c o2 ob ol = ()
+
 let one_op_inter_base_left_a l a b c o2 ob ol = ()
 let one_op_inter_base_left_b l a b c o2 ob ol = ()
 let one_op_inter_base_left_ne l a b c o2 ob ol = ()
+
 let one_op_inter_right_a l a b c o2 ob ol o = ()
 let one_op_inter_right_b l a b c o2 ob ol o = ()
 let one_op_inter_right_ne l a b c o2 ob ol o = ()
+
 let one_op_inter_left_a l a b c o2 ob ol o = ()
 let one_op_inter_left_b l a b c o2 ob ol o = ()
 let one_op_inter_left_ne l a b c o2 ob ol o = ()
+
 let one_op_inter_lca_a l a b c o2 ol oi o = ()
 let one_op_inter_lca_b l a b c o2 ol oi o = ()
 let one_op_inter_lca_ne l a b c o2 ol oi o = ()
+
+let zero_op_inter_base_right_a l a b c ob ol = ()
+let zero_op_inter_base_right_b l a b c ob ol = ()
+let zero_op_inter_base_right_ne l a b c ob ol = ()
+
+let zero_op_inter_base_left_a l a b c ob ol = ()
+let zero_op_inter_base_left_b l a b c ob ol = ()
+let zero_op_inter_base_left_ne l a b c ob ol = ()
+
+let zero_op_inter_right_a l a b c ob ol o = ()
+let zero_op_inter_right_b l a b c ob ol o = ()
+let zero_op_inter_right_ne l a b c ob ol o = ()
+
+let zero_op_inter_left_a l a b c ob ol o = ()
+let zero_op_inter_left_b l a b c ob ol o = ()
+let zero_op_inter_left_ne l a b c ob ol o = ()
+
+let zero_op_inter_lca_v1_a l a b c ol = ()
+let zero_op_inter_lca_v1_b l a b c ol = ()
+
+let zero_op_inter_lca_v2_a l a b c ol oi = ()
+let zero_op_inter_lca_v2_b l a b c ol oi = ()
+let zero_op_inter_lca_v2_ne l a b c ol oi = ()
+
+let comm_ind_right_a l a b o1 o2 o2' = ()
+let comm_ind_right_b l a b o1 o2 o2' = ()
+let comm_ind_right_ne l a b o1 o2 o2' = ()
+
+let comm_ind_left_a l a b o1 o2 o1' = ()
+let comm_ind_left_b l a b o1 o2 o1' = ()
+let comm_ind_left_ne l a b o1 o2 o1' = ()
+
+let comm_ind_lca_a l ol o1 o2 = ()
+let comm_ind_lca_b l ol o1 o2 = ()
+let comm_ind_lca_ne l ol o1 o2 = ()
+
+let comm_base o1 o2 t = ()
+
+let comm_inter_base_right_a l a b c o1 o2 ob ol = ()
+let comm_inter_base_right_b l a b c o1 o2 ob ol = ()
+let comm_inter_base_right_ne l a b c o1 o2 ob ol = ()
+
+let comm_inter_base_left_a l a b c o1 o2 ob ol = ()
+let comm_inter_base_left_b l a b c o1 o2 ob ol = ()
+let comm_inter_base_left_ne l a b c o1 o2 ob ol = ()
+
+let comm_inter_right_a l a b c o1 o2 ob ol o = ()
+let comm_inter_right_b l a b c o1 o2 ob ol o = ()
+let comm_inter_right_ne l a b c o1 o2 ob ol o = ()
+
+let comm_inter_left_a l a b c o1 o2 ob ol o = ()
+let comm_inter_left_b l a b c o1 o2 ob ol o = ()
+let comm_inter_left_ne l a b c o1 o2 ob ol o = ()
+
+let comm_inter_lca_a l a b c o1 o2 ol = ()
+let comm_inter_lca_b l a b c o1 o2 ol = ()
+let comm_inter_lca_ne l a b c o1 o2 ol = ()
