interface/Polymorphic_gmap.fsti
@@ -876,7 +876,7 @@ val one_op_inter_lca_ne (l a b c:concrete_st) (o2 ol oi o:op_t)
                     Fst_then_snd? (rc o oi) /\ 
                     ~ (get_key ol = get_key oi /\ get_key o2 = get_key oi /\
                        (is_alpha_op oi /\ is_alpha_op ol /\ is_alpha_op o2 /\ is_alpha_op o /\ Fst_then_snd? (rc_a (get_op_a o) (get_op_a ol)) /\ Fst_then_snd? (rc_a (get_op_a o) (get_op_a oi))) /\
-                       (is_beta_op oi /\ is_beta_op ol /\ is_beta_op o2 /\ is_beta_op o /\ Fst_then_snd? (rc_b (get_op_b o) (get_op_b ol)) /\ Fst_then_snd? (rc_b (get_op_a o) (get_op_a oi)))) /\
+                       (is_beta_op oi /\ is_beta_op ol /\ is_beta_op o2 /\ is_beta_op o /\ Fst_then_snd? (rc_b (get_op_b o) (get_op_b ol)) /\ Fst_then_snd? (rc_b (get_op_b o) (get_op_b oi)))) /\
                     eq (merge (do l oi) (do a oi) (do (do b oi) o2)) (do (do c oi) o2) /\
                     eq (merge (do l ol) (do a ol) (do (do b ol) o2)) (do (do c ol) o2))
           (ensures eq (merge (do (do l oi) ol) (do (do a oi) ol) (do (do (do b oi) ol) o2)) (do (do (do c oi) ol) o2)) 
@@ -899,53 +899,559 @@ let one_op_inter_lca (l a b c:concrete_st) (o2 ol oi o:op_t)
 // because we proved that e_i^l rcp eb is not possible.
 //e_i^l vis eb is not possible
 // so either eb rcp e_i^l or eb rct e_i^l is possible
-val one_op_inter_right_a (l a b c:concrete_st_a) (o2 ob ol:op_a) 
-  : Lemma (requires Fst_then_snd? (rc_a ob ol) /\
-                    distinct_ops o2 ob /\ distinct_ops o2 ol /\ distinct_ops ob ol /\
-                    eq_a (merge_a (do_a l ol) (do_a a ol) (do_a (do_a b ol) o2)) (do_a (do_a c ol) o2) /\
-                    eq_a (merge_a l a (do_a b o2)) (do_a c o2) /\
+val zero_op_inter_base_right_a (l a b c:concrete_st_a) (ob ol:op_a) 
+  : Lemma (requires Fst_then_snd? (rc_a ob ol) /\ distinct_ops ob ol /\
+                    eq_a (merge_a (do_a l ol) (do_a a ol) (do_a b ol)) (do_a c ol) /\
+                    eq_a (merge_a l a b) c /\
                     eq_a (merge_a l (do_a a ol) (do_a b ob)) (do_a (do_a c ob) ol)) //***EXTRA***
-          (ensures eq_a (merge_a (do_a l ol) (do_a a ol) (do_a (do_a (do_a b ob) ol) o2)) (do_a (do_a (do_a c ob) ol) o2)) 
+          (ensures eq_a (merge_a (do_a l ol) (do_a a ol) (do_a (do_a b ob) ol)) (do_a (do_a c ob) ol))
 
-val one_op_inter_right_b (l a b c:concrete_st_b) (o2 ob ol:op_b) 
-  : Lemma (requires Fst_then_snd? (rc_b ob ol) /\
-                    distinct_ops o2 ob /\ distinct_ops o2 ol /\ distinct_ops ob ol /\
-                    eq_b (merge_b (do_b l ol) (do_b a ol) (do_b (do_b b ol) o2)) (do_b (do_b c ol) o2) /\
-                    eq_b (merge_b l a (do_b b o2)) (do_b c o2) /\
+val zero_op_inter_base_right_b (l a b c:concrete_st_b) (ob ol:op_b) 
+  : Lemma (requires Fst_then_snd? (rc_b ob ol) /\ distinct_ops ob ol /\
+                    eq_b (merge_b (do_b l ol) (do_b a ol) (do_b b ol)) (do_b c ol) /\
+                    eq_b (merge_b l a b) c /\
                     eq_b (merge_b l (do_b a ol) (do_b b ob)) (do_b (do_b c ob) ol)) //***EXTRA***
-          (ensures eq_b (merge_b (do_b l ol) (do_b a ol) (do_b (do_b (do_b b ob) ol) o2)) (do_b (do_b (do_b c ob) ol) o2)) 
+          (ensures eq_b (merge_b (do_b l ol) (do_b a ol) (do_b (do_b b ob) ol)) (do_b (do_b c ob) ol))
 
-val one_op_inter_right_ne (l a b c:concrete_st) (o2 ob ol:op_t) 
-  : Lemma (requires Fst_then_snd? (rc ob ol) /\
-                    distinct_ops o2 ob /\ distinct_ops o2 ol /\ distinct_ops ob ol /\
-                    ~ (get_key ol = get_key ob && get_key o2 = get_key ob /\
-                       (is_alpha_op ob && is_alpha_op ol && is_alpha_op o2 && Fst_then_snd? (rc_a (get_op_a ob) (get_op_a ol))) /\
-                       (is_beta_op ob && is_beta_op ol && is_beta_op o2 && Fst_then_snd? (rc_b (get_op_b ob) (get_op_b ol)))) /\
-                    eq (merge (do l ol) (do a ol) (do (do b ol) o2)) (do (do c ol) o2) /\
-                    eq (merge l a (do b o2)) (do c o2) /\
+val zero_op_inter_base_right_ne (l a b c:concrete_st) (ob ol:op_t) 
+  : Lemma (requires Fst_then_snd? (rc ob ol) /\ distinct_ops ob ol /\
+                    ~ (get_key ol = get_key ob /\
+                       (is_alpha_op ob /\ is_alpha_op ol /\ Fst_then_snd? (rc_a (get_op_a ob) (get_op_a ol))) /\
+                       (is_beta_op ob /\ is_beta_op ol /\ Fst_then_snd? (rc_b (get_op_b ob) (get_op_b ol)))) /\
+                    eq (merge (do l ol) (do a ol) (do b ol)) (do c ol) /\
+                    eq (merge l a b) c /\
                     eq (merge l (do a ol) (do b ob)) (do (do c ob) ol)) //***EXTRA***
-          (ensures eq (merge (do l ol) (do a ol) (do (do (do b ob) ol) o2)) (do (do (do c ob) ol) o2))
+          (ensures eq (merge (do l ol) (do a ol) (do (do b ob) ol)) (do (do c ob) ol)) 
           
-let one_op_inter_right (l a b c:concrete_st) (o2 ob ol:op_t) 
-  : Lemma (requires Fst_then_snd? (rc ob ol) /\
-                    distinct_ops o2 ob /\ distinct_ops o2 ol /\ distinct_ops ob ol /\
-                    eq (merge (do l ol) (do a ol) (do (do b ol) o2)) (do (do c ol) o2) /\
-                    eq (merge l a (do b o2)) (do c o2) /\
+let zero_op_inter_base_right (l a b c:concrete_st) (ob ol:op_t) 
+  : Lemma (requires Fst_then_snd? (rc ob ol) /\ distinct_ops ob ol /\
+                    eq (merge (do l ol) (do a ol) (do b ol)) (do c ol) /\
+                    eq (merge l a b) c /\
                     eq (merge l (do a ol) (do b ob)) (do (do c ob) ol)) //***EXTRA***
-          (ensures eq (merge (do l ol) (do a ol) (do (do (do b ob) ol) o2)) (do (do (do c ob) ol) o2)) =
+          (ensures eq (merge (do l ol) (do a ol) (do (do b ob) ol)) (do (do c ob) ol)) =
   let k = get_key ob in
-  if get_key ol = k && get_key o2 = k && is_alpha_op ob && is_alpha_op ol && is_alpha_op o2 && Fst_then_snd? (rc_a (get_op_a ob) (get_op_a ol)) then
-    one_op_inter_base_right_a (sel_a l k) (sel_a a k) (sel_a b k) (sel_a c k) (get_op_a o2) (get_op_a ob) (get_op_a ol)
-  else if get_key ol = k && get_key o2 = k && is_beta_op ob && is_beta_op ol && is_beta_op o2 && Fst_then_snd? (rc_b (get_op_b ob) (get_op_b ol)) then
-    one_op_inter_base_right_b (sel_b l k) (sel_b a k) (sel_b b k) (sel_b c k) (get_op_b o2) (get_op_b ob) (get_op_b ol)
-  else one_op_inter_base_right_ne l a b c o2 ob ol
-  
+  if get_key ol = k && is_alpha_op ob && is_alpha_op ol && Fst_then_snd? (rc_a (get_op_a ob) (get_op_a ol)) then
+    zero_op_inter_base_right_a (sel_a l k) (sel_a a k) (sel_a b k) (sel_a c k) (get_op_a ob) (get_op_a ol)
+  else if get_key ol = k && is_beta_op ob && is_beta_op ol && Fst_then_snd? (rc_b (get_op_b ob) (get_op_b ol)) then
+    zero_op_inter_base_right_b (sel_b l k) (sel_b a k) (sel_b b k) (sel_b c k) (get_op_b ob) (get_op_b ol)
+  else zero_op_inter_base_right_ne l a b c ob ol
 
+val zero_op_inter_base_left_a (l a b c:concrete_st_a) (ob ol:op_a) 
+  : Lemma (requires Fst_then_snd? (rc_a ob ol) /\ distinct_ops ob ol /\
+                    eq_a (merge_a (do_a l ol) (do_a a ol) (do_a b ol)) (do_a c ol) /\
+                    eq_a (merge_a l a b) c /\
+                    eq_a (merge_a l (do_a a ob) (do_a b ol)) (do_a (do_a c ob) ol)) //***EXTRA***
+          (ensures eq_a (merge_a (do_a l ol) (do_a (do_a a ob) ol) (do_a b ol)) (do_a (do_a c ob) ol))
 
+val zero_op_inter_base_left_b (l a b c:concrete_st_b) (ob ol:op_b) 
+  : Lemma (requires Fst_then_snd? (rc_b ob ol) /\ distinct_ops ob ol /\
+                    eq_b (merge_b (do_b l ol) (do_b a ol) (do_b b ol)) (do_b c ol) /\
+                    eq_b (merge_b l a b) c /\
+                    eq_b (merge_b l (do_b a ob) (do_b b ol)) (do_b (do_b c ob) ol)) //***EXTRA***
+          (ensures eq_b (merge_b (do_b l ol) (do_b (do_b a ob) ol) (do_b b ol)) (do_b (do_b c ob) ol))
 
+val zero_op_inter_base_left_ne (l a b c:concrete_st) (ob ol:op_t) 
+  : Lemma (requires Fst_then_snd? (rc ob ol) /\ distinct_ops ob ol /\
+                    ~ (get_key ol = get_key ob /\
+                       (is_alpha_op ob /\ is_alpha_op ol /\ Fst_then_snd? (rc_a (get_op_a ob) (get_op_a ol))) /\
+                       (is_beta_op ob /\ is_beta_op ol /\ Fst_then_snd? (rc_b (get_op_b ob) (get_op_b ol)))) /\
+                    eq (merge (do l ol) (do a ol) (do b ol)) (do c ol) /\
+                    eq (merge l a b) c /\
+                    eq (merge l (do a ob) (do b ol)) (do (do c ob) ol)) //***EXTRA***
+          (ensures eq (merge (do l ol) (do (do a ob) ol) (do b ol)) (do (do c ob) ol)) 
+          
+let zero_op_inter_base_left (l a b c:concrete_st) (ob ol:op_t) 
+  : Lemma (requires Fst_then_snd? (rc ob ol) /\ distinct_ops ob ol /\
+                    eq (merge (do l ol) (do a ol) (do b ol)) (do c ol) /\
+                    eq (merge l a b) c /\
+                    eq (merge l (do a ob) (do b ol)) (do (do c ob) ol)) //***EXTRA***
+          (ensures eq (merge (do l ol) (do (do a ob) ol) (do b ol)) (do (do c ob) ol)) =
+  let k = get_key ob in
+  if get_key ol = k && is_alpha_op ob && is_alpha_op ol && Fst_then_snd? (rc_a (get_op_a ob) (get_op_a ol)) then
+    zero_op_inter_base_left_a (sel_a l k) (sel_a a k) (sel_a b k) (sel_a c k) (get_op_a ob) (get_op_a ol)
+  else if get_key ol = k && is_beta_op ob && is_beta_op ol && Fst_then_snd? (rc_b (get_op_b ob) (get_op_b ol)) then
+    zero_op_inter_base_left_b (sel_b l k) (sel_b a k) (sel_b b k) (sel_b c k) (get_op_b ob) (get_op_b ol)
+  else zero_op_inter_base_left_ne l a b c ob ol
 
+val zero_op_inter_right_a (l a b c:concrete_st_a) (ob ol o:op_a) 
+  : Lemma (requires Fst_then_snd? (rc_a ob ol) /\
+                    distinct_ops o ob /\ distinct_ops o ol /\ distinct_ops o ol /\ distinct_ops ob ol /\ 
+                    get_rid o <> get_rid ol (*o,ol must be concurrent*) /\
+                    (~ (Either? (rc_a o ob)) \/ Fst_then_snd? (rc_a o ol)) /\
+                    eq_a (merge_a (do_a l ol) (do_a a ol) (do_a (do_a b ob) ol)) (do_a (do_a c ob) ol))
+          (ensures eq_a (merge_a (do_a l ol) (do_a a ol) (do_a (do_a (do_a b o) ob) ol)) (do_a (do_a (do_a c o) ob) ol))
 
+val zero_op_inter_right_b (l a b c:concrete_st_b) (ob ol o:op_b) 
+  : Lemma (requires Fst_then_snd? (rc_b ob ol) /\
+                    distinct_ops o ob /\ distinct_ops o ol /\ distinct_ops o ol /\ distinct_ops ob ol /\
+                    get_rid o <> get_rid ol (*o,ol must be concurrent*) /\
+                    (~ (Either? (rc_b o ob)) \/ Fst_then_snd? (rc_b o ol)) /\
+                    eq_b (merge_b (do_b l ol) (do_b a ol) (do_b (do_b b ob) ol)) (do_b (do_b c ob) ol))
+          (ensures eq_b (merge_b (do_b l ol) (do_b a ol) (do_b (do_b (do_b b o) ob) ol)) (do_b (do_b (do_b c o) ob) ol))
 
+val zero_op_inter_right_ne (l a b c:concrete_st) (ob ol o:op_t) 
+  : Lemma (requires Fst_then_snd? (rc ob ol) /\
+                    distinct_ops o ob /\ distinct_ops o ol /\ distinct_ops o ol /\ distinct_ops ob ol /\
+                    get_rid o <> get_rid ol (*o,ol must be concurrent*) /\
+                    ~ (get_key o = get_key ob && get_key o = get_key ol /\
+                       (is_alpha_op ob && is_alpha_op ol && is_alpha_op o && Fst_then_snd? (rc_a (get_op_a ob) (get_op_a ol))) /\
+                       (is_beta_op ob && is_beta_op ol && is_alpha_op o && Fst_then_snd? (rc_b (get_op_b ob) (get_op_b ol)))) /\
+                    (~ (Either? (rc o ob)) \/ Fst_then_snd? (rc o ol)) /\
+                    eq (merge (do l ol) (do a ol) (do (do b ob) ol)) (do (do c ob) ol))
+          (ensures eq (merge (do l ol) (do a ol) (do (do (do b o) ob) ol)) (do (do (do c o) ob) ol))
+          
+let zero_op_inter_right (l a b c:concrete_st) (ob ol o:op_t) 
+  : Lemma (requires Fst_then_snd? (rc ob ol) /\
+                    distinct_ops o ob /\ distinct_ops o ol /\ distinct_ops o ol /\ distinct_ops ob ol /\
+                    get_rid o <> get_rid ol (*o,ol must be concurrent*) /\
+                    (~ (Either? (rc o ob)) \/ Fst_then_snd? (rc o ol)) /\
+                    eq (merge (do l ol) (do a ol) (do (do b ob) ol)) (do (do c ob) ol))
+          (ensures eq (merge (do l ol) (do a ol) (do (do (do b o) ob) ol)) (do (do (do c o) ob) ol)) =
+  let k = get_key o in
+  if get_key ob = k && get_key ol = k && is_alpha_op o && is_alpha_op ob && is_alpha_op ol && Fst_then_snd? (rc_a (get_op_a ob) (get_op_a ol)) then
+    zero_op_inter_right_a (sel_a l k) (sel_a a k) (sel_a b k) (sel_a c k) (get_op_a ob) (get_op_a ol) (get_op_a o)
+  else if get_key ol = k && is_beta_op ob && is_beta_op ol && Fst_then_snd? (rc_b (get_op_b ob) (get_op_b ol)) then
+    zero_op_inter_right_b (sel_b l k) (sel_b a k) (sel_b b k) (sel_b c k) (get_op_b ob) (get_op_b ol) (get_op_b o)
+  else zero_op_inter_right_ne l a b c ob ol o
+
+val zero_op_inter_left_a (l a b c:concrete_st_a) (ob ol o:op_a) 
+  : Lemma (requires Fst_then_snd? (rc_a ob ol) /\
+                    distinct_ops o ob /\ distinct_ops o ol /\ distinct_ops o ol /\ distinct_ops ob ol /\ 
+                    get_rid o <> get_rid ol (*o,ol must be concurrent*) /\
+                    (~ (Either? (rc_a o ob)) \/ Fst_then_snd? (rc_a o ol)) /\
+                    eq_a (merge_a (do_a l ol) (do_a (do_a a ob) ol) (do_a b ol)) (do_a (do_a c ob) ol))
+          (ensures eq_a (merge_a (do_a l ol) (do_a (do_a (do_a a o) ob) ol) (do_a b ol)) (do_a (do_a (do_a c o) ob) ol)) 
+
+val zero_op_inter_left_b (l a b c:concrete_st_b) (ob ol o:op_b) 
+  : Lemma (requires Fst_then_snd? (rc_b ob ol) /\
+                    distinct_ops o ob /\ distinct_ops o ol /\ distinct_ops o ol /\ distinct_ops ob ol /\
+                    get_rid o <> get_rid ol (*o,ol must be concurrent*) /\
+                    (~ (Either? (rc_b o ob)) \/ Fst_then_snd? (rc_b o ol)) /\
+                    eq_b (merge_b (do_b l ol) (do_b (do_b a ob) ol) (do_b b ol)) (do_b (do_b c ob) ol))
+          (ensures eq_b (merge_b (do_b l ol) (do_b (do_b (do_b a o) ob) ol) (do_b b ol)) (do_b (do_b (do_b c o) ob) ol)) 
+
+val zero_op_inter_left_ne (l a b c:concrete_st) (ob ol o:op_t) 
+  : Lemma (requires Fst_then_snd? (rc ob ol) /\
+                    distinct_ops o ob /\ distinct_ops o ol /\ distinct_ops o ol /\ distinct_ops ob ol /\
+                    get_rid o <> get_rid ol (*o,ol must be concurrent*) /\
+                    ~ (get_key o = get_key ob && get_key o = get_key ol /\
+                       (is_alpha_op ob && is_alpha_op ol && is_alpha_op o && Fst_then_snd? (rc_a (get_op_a ob) (get_op_a ol))) /\
+                       (is_beta_op ob && is_beta_op ol && is_alpha_op o && Fst_then_snd? (rc_b (get_op_b ob) (get_op_b ol)))) /\
+                    (~ (Either? (rc o ob)) \/ Fst_then_snd? (rc o ol)) /\
+                    eq (merge (do l ol) (do (do a ob) ol) (do b ol)) (do (do c ob) ol))
+          (ensures eq (merge (do l ol) (do (do (do a o) ob) ol) (do b ol)) (do (do (do c o) ob) ol)) 
+          
+let zero_op_inter_left (l a b c:concrete_st) (ob ol o:op_t) 
+  : Lemma (requires Fst_then_snd? (rc ob ol) /\
+                    distinct_ops o ob /\ distinct_ops o ol /\ distinct_ops o ol /\ distinct_ops ob ol /\
+                    get_rid o <> get_rid ol (*o,ol must be concurrent*) /\
+                    (~ (Either? (rc o ob)) \/ Fst_then_snd? (rc o ol)) /\
+                    eq (merge (do l ol) (do (do a ob) ol) (do b ol)) (do (do c ob) ol))
+          (ensures eq (merge (do l ol) (do (do (do a o) ob) ol) (do b ol)) (do (do (do c o) ob) ol)) =
+  let k = get_key o in
+  if get_key ob = k && get_key ol = k && is_alpha_op o && is_alpha_op ob && is_alpha_op ol && Fst_then_snd? (rc_a (get_op_a ob) (get_op_a ol)) then
+    zero_op_inter_left_a (sel_a l k) (sel_a a k) (sel_a b k) (sel_a c k) (get_op_a ob) (get_op_a ol) (get_op_a o)
+  else if get_key ol = k && is_beta_op ob && is_beta_op ol && Fst_then_snd? (rc_b (get_op_b ob) (get_op_b ol)) then
+    zero_op_inter_left_b (sel_b l k) (sel_b a k) (sel_b b k) (sel_b c k) (get_op_b ob) (get_op_b ol) (get_op_b o)
+  else zero_op_inter_left_ne l a b c ob ol o
+
+val zero_op_inter_lca_v1_a (l a b c:concrete_st_a) (ol:op_a)
+  : Lemma (requires (exists o'. Fst_then_snd? (rc_a o' ol)) /\ eq_a (merge_a l a b) c)
+          (ensures eq_a (merge_a (do_a l ol) (do_a a ol) (do_a b ol)) (do_a c ol))
+
+val zero_op_inter_lca_v1_b (l a b c:concrete_st_b) (ol:op_b)
+  : Lemma (requires (exists o'. Fst_then_snd? (rc_b o' ol)) /\ eq_b (merge_b l a b) c)
+          (ensures eq_b (merge_b (do_b l ol) (do_b a ol) (do_b b ol)) (do_b c ol))
+          
+let zero_op_inter_lca_v1 (l a b c:concrete_st) (ol:op_t)
+  : Lemma (requires (exists o'. Fst_then_snd? (rc o' ol)) /\ eq (merge l a b) c)
+          (ensures eq (merge (do l ol) (do a ol) (do b ol)) (do c ol)) =
+  let k = get_key ol in
+  if is_alpha_op ol then zero_op_inter_lca_v1_a (sel_a l k) (sel_a a k) (sel_a b k) (sel_a c k) (get_op_a ol)
+  else zero_op_inter_lca_v1_b (sel_b l k) (sel_b a k) (sel_b b k) (sel_b c k) (get_op_b ol)
+
+val zero_op_inter_lca_v2_a (l a b c:concrete_st_a) (ol oi:op_a)
+  : Lemma (requires (exists o'. Fst_then_snd? (rc_a o' ol)) /\
+                    (exists o'. Fst_then_snd? (rc_a o' oi)) /\
+                    eq_a (merge_a (do_a l oi) (do_a a oi) (do_a b oi)) (do_a c oi)  /\
+                    eq_a (merge_a (do_a l ol) (do_a a ol) (do_a b ol)) (do_a c ol))
+          (ensures eq_a (merge_a (do_a (do_a l oi) ol) (do_a (do_a a oi) ol) (do_a (do_a b oi) ol)) (do_a (do_a c oi) ol))
+
+val zero_op_inter_lca_v2_b (l a b c:concrete_st_b) (ol oi:op_b)
+  : Lemma (requires (exists o'. Fst_then_snd? (rc_b o' ol)) /\ 
+                    (exists o'. Fst_then_snd? (rc_b o' oi)) /\ 
+                    eq_b (merge_b (do_b l oi) (do_b a oi) (do_b b oi)) (do_b c oi)  /\
+                    eq_b (merge_b (do_b l ol) (do_b a ol) (do_b b ol)) (do_b c ol))
+          (ensures eq_b (merge_b (do_b (do_b l oi) ol) (do_b (do_b a oi) ol) (do_b (do_b b oi) ol)) (do_b (do_b c oi) ol))
+
+val zero_op_inter_lca_v2_ne (l a b c:concrete_st) (ol oi:op_t)
+  : Lemma (requires (exists o. Fst_then_snd? (rc o ol)) /\ 
+                    (exists o. Fst_then_snd? (rc o oi)) /\
+                    ~ (get_key ol = get_key oi /\
+                       (is_alpha_op ol /\ is_alpha_op oi) /\
+                       (is_beta_op ol /\ is_beta_op oi)) /\
+                    eq (merge (do l oi) (do a oi) (do b oi)) (do c oi)  /\
+                    eq (merge (do l ol) (do a ol) (do b ol)) (do c ol))
+          (ensures eq (merge (do (do l oi) ol) (do (do a oi) ol) (do (do b oi) ol)) (do (do c oi) ol))
+          
+let zero_op_inter_lca_v2 (l a b c:concrete_st) (ol oi:op_t)
+  : Lemma (requires (exists o. Fst_then_snd? (rc o ol)) /\ 
+                    (exists o. Fst_then_snd? (rc o oi)) /\
+                    eq (merge (do l oi) (do a oi) (do b oi)) (do c oi)  /\
+                    eq (merge (do l ol) (do a ol) (do b ol)) (do c ol))
+          (ensures eq (merge (do (do l oi) ol) (do (do a oi) ol) (do (do b oi) ol)) (do (do c oi) ol)) =
+  let k = get_key oi in
+  if get_key ol = k && is_alpha_op ol && is_alpha_op oi then zero_op_inter_lca_v2_a (sel_a l k) (sel_a a k) (sel_a b k) (sel_a c k) (get_op_a ol) (get_op_a oi)
+  else if get_key ol = k && is_beta_op ol && is_beta_op oi then zero_op_inter_lca_v2_b (sel_b l k) (sel_b a k) (sel_b b k) (sel_b c k) (get_op_b ol) (get_op_b oi)
+  else zero_op_inter_lca_v2_ne l a b c ol oi
+
+(* 2 op Comm  *)
+///////////////////
+
+val comm_ind_right_a (l a b:concrete_st_a) (o1 o2 o2':op_a)
+  : Lemma (requires Either? (rc_a o1 o2) /\
+                    (Fst_then_snd? (rc_a o2' o1) ==> (eq_a (merge_a l (do_a a o1) (do_a b o2')) (do_a (merge_a l a (do_a b o2')) o1))) /\
+                    ~ (Fst_then_snd? (rc_a o1 o2')) /\
+                    eq_a (merge_a l (do_a a o1) (do_a b o2)) (do_a (do_a (merge_a l a b) o2) o1))
+          (ensures eq_a (merge_a l (do_a a o1) (do_a (do_a b o2') o2)) (do_a (do_a (merge_a l a (do_a b o2')) o2) o1))
+
+val comm_ind_right_b (l a b:concrete_st_b) (o1 o2 o2':op_b)
+  : Lemma (requires Either? (rc_b o1 o2) /\
+                    (Fst_then_snd? (rc_b o2' o1) ==> (eq_b (merge_b l (do_b a o1) (do_b b o2')) (do_b (merge_b l a (do_b b o2')) o1))) /\
+                    ~ (Fst_then_snd? (rc_b o1 o2')) /\
+                    eq_b (merge_b l (do_b a o1) (do_b b o2)) (do_b (do_b (merge_b l a b) o2) o1))
+          (ensures eq_b (merge_b l (do_b a o1) (do_b (do_b b o2') o2)) (do_b (do_b (merge_b l a (do_b b o2')) o2) o1))
+
+val comm_ind_right_ne (l a b:concrete_st) (o1 o2 o2':op_t)
+  : Lemma (requires Either? (rc o1 o2) /\ 
+                    distinct_ops o1 o2 /\ distinct_ops o1 o2' /\ distinct_ops o2 o2' /\
+                    ~ (get_key o2 = get_key o2' && get_key o1 = get_key o2' /\
+                       (is_alpha_op o1 /\ is_alpha_op o2 /\ is_alpha_op o2') /\
+                       (is_beta_op o1 /\ is_beta_op o2 /\ is_beta_op o2')) /\
+                    eq (merge l (do a o1) (do b o2)) (do (do (merge l a b) o2) o1) /\
+                    (Fst_then_snd? (rc o2' o1) ==> (eq (merge l (do a o1) (do b o2')) (do (merge l a (do b o2')) o1))) /\
+                    ~ (exists o3 a'. eq (do a o1) (do a' o3) /\ distinct_ops o2 o3 /\ Fst_then_snd? (rc o2 o3)) /\
+                    ~ (Fst_then_snd? (rc o1 o2')) /\
+                    ~ (exists o3 b'. eq (do (do b o2') o2) (do b' o3) /\ distinct_ops o1 o3 /\ Fst_then_snd? (rc o1 o3)) /\
+                    ~ (exists o3 b'. eq (do b o2) (do b' o3) /\ distinct_ops o1 o3 /\ Fst_then_snd? (rc o1 o3)))  
+          (ensures eq (merge l (do a o1) (do (do b o2') o2)) (do (do (merge l a (do b o2')) o2) o1))
+                    
+let comm_ind_right (l a b:concrete_st) (o1 o2 o2':op_t)
+  : Lemma (requires Either? (rc o1 o2) /\ 
+                    distinct_ops o1 o2 /\ distinct_ops o1 o2' /\ distinct_ops o2 o2' /\
+                    eq (merge l (do a o1) (do b o2)) (do (do (merge l a b) o2) o1) /\
+                    (Fst_then_snd? (rc o2' o1) ==> (eq (merge l (do a o1) (do b o2')) (do (merge l a (do b o2')) o1))) /\
+                    ~ (exists o3 a'. eq (do a o1) (do a' o3) /\ distinct_ops o2 o3 /\ Fst_then_snd? (rc o2 o3)) /\
+                    ~ (Fst_then_snd? (rc o1 o2')) /\
+                    ~ (exists o3 b'. eq (do (do b o2') o2) (do b' o3) /\ distinct_ops o1 o3 /\ Fst_then_snd? (rc o1 o3)) /\
+                    ~ (exists o3 b'. eq (do b o2) (do b' o3) /\ distinct_ops o1 o3 /\ Fst_then_snd? (rc o1 o3)))                    
+          (ensures eq (merge l (do a o1) (do (do b o2') o2)) (do (do (merge l a (do b o2')) o2) o1)) =
+  let k = get_key o2' in
+  if get_key o2 = k && get_key o1 = k && is_alpha_op o1 && is_alpha_op o2' && is_alpha_op o2 && Either? (rc_a (get_op_a o1) (get_op_a o2)) then
+    comm_ind_right_a (sel_a l k) (sel_a a k) (sel_a b k) (get_op_a o1) (get_op_a o2) (get_op_a o2')
+  else if get_key o2 = k && get_key o1 = k && is_beta_op o1 && is_beta_op o2' && is_beta_op o2 && Either? (rc_b (get_op_b o1) (get_op_b o2)) then 
+    comm_ind_right_b (sel_b l k) (sel_b a k) (sel_b b k) (get_op_b o1) (get_op_b o2) (get_op_b o2')
+  else comm_ind_right_ne l a b o1 o2 o2'
+
+val comm_ind_left_a (l a b:concrete_st_a) (o1 o2 o1':op_a)
+  : Lemma (requires Either? (rc_a o1 o2) /\
+                    (Fst_then_snd? (rc_a o1' o2) ==> (eq_a (merge_a l (do_a a o1') (do_a b o2)) (do_a (merge_a l (do_a a o1') b) o2))) /\
+                    ~ (Fst_then_snd? (rc_a o2 o1')) /\
+                    eq_a (merge_a l (do_a a o1) (do_a b o2)) (do_a (do_a (merge_a l a b) o2) o1))
+          (ensures eq_a (merge_a l (do_a (do_a a o1') o1) (do_a b o2)) (do_a (do_a (merge_a l (do_a a o1') b) o2) o1))
+
+val comm_ind_left_b (l a b:concrete_st_b) (o1 o2 o1':op_b)
+  : Lemma (requires Either? (rc_b o1 o2) /\
+                    (Fst_then_snd? (rc_b o1' o2) ==> (eq_b (merge_b l (do_b a o1') (do_b b o2)) (do_b (merge_b l (do_b a o1') b) o2))) /\
+                    ~ (Fst_then_snd? (rc_b o2 o1')) /\
+                    eq_b (merge_b l (do_b a o1) (do_b b o2)) (do_b (do_b (merge_b l a b) o2) o1))
+          (ensures eq_b (merge_b l (do_b (do_b a o1') o1) (do_b b o2)) (do_b (do_b (merge_b l (do_b a o1') b) o2) o1))
+
+val comm_ind_left_ne (l a b:concrete_st) (o1 o2 o1':op_t)
+  : Lemma (requires Either? (rc o1 o2) /\ 
+                    distinct_ops o1 o2 /\ distinct_ops o1 o1' /\ distinct_ops o2 o1' /\
+                    ~ (get_key o2 = get_key o1' && get_key o1 = get_key o1' /\
+                       (is_alpha_op o1 /\ is_alpha_op o2 /\ is_alpha_op o1') /\
+                       (is_beta_op o1 /\ is_beta_op o2 /\ is_beta_op o1')) /\
+                    eq (merge l (do a o1) (do b o2)) (do (do (merge l a b) o2) o1) /\
+                    (Fst_then_snd? (rc o1' o2) ==> (eq (merge l (do a o1') (do b o2)) (do (merge l (do a o1') b) o2))) /\
+                    ~ (exists o3 a'. eq (do a o1) (do a' o3) /\ distinct_ops o2 o3 /\ Fst_then_snd? (rc o2 o3)) /\
+                    ~ (Fst_then_snd? (rc o2 o1')) /\
+                    ~ (exists o3 b'. eq (do (do b o1') o2) (do b' o3) /\ distinct_ops o1 o3 /\ Fst_then_snd? (rc o1 o3)) /\
+                    ~ (exists o3 b'. eq (do b o2) (do b' o3) /\ distinct_ops o1 o3 /\ Fst_then_snd? (rc o1 o3)))                    
+          (ensures eq (merge l (do (do a o1') o1) (do b o2)) (do (do (merge l (do a o1') b) o2) o1))
+                    
+let comm_ind_left (l a b:concrete_st) (o1 o2 o1':op_t)
+  : Lemma (requires Either? (rc o1 o2) /\ 
+                    distinct_ops o1 o2 /\ distinct_ops o1 o1' /\ distinct_ops o2 o1' /\
+                    eq (merge l (do a o1) (do b o2)) (do (do (merge l a b) o2) o1) /\
+                    (Fst_then_snd? (rc o1' o2) ==> (eq (merge l (do a o1') (do b o2)) (do (merge l (do a o1') b) o2))) /\
+                    ~ (exists o3 a'. eq (do a o1) (do a' o3) /\ distinct_ops o2 o3 /\ Fst_then_snd? (rc o2 o3)) /\
+                    ~ (Fst_then_snd? (rc o2 o1')) /\
+                    ~ (exists o3 b'. eq (do (do b o1') o2) (do b' o3) /\ distinct_ops o1 o3 /\ Fst_then_snd? (rc o1 o3)) /\
+                    ~ (exists o3 b'. eq (do b o2) (do b' o3) /\ distinct_ops o1 o3 /\ Fst_then_snd? (rc o1 o3)))                    
+          (ensures eq (merge l (do (do a o1') o1) (do b o2)) (do (do (merge l (do a o1') b) o2) o1)) =
+  let k = get_key o1' in
+  if get_key o2 = k && get_key o1 = k && is_alpha_op o1 && is_alpha_op o1' && is_alpha_op o2 && Either? (rc_a (get_op_a o1) (get_op_a o2)) then
+    comm_ind_left_a (sel_a l k) (sel_a a k) (sel_a b k) (get_op_a o1) (get_op_a o2) (get_op_a o1')
+  else if get_key o2 = k && get_key o1 = k && is_beta_op o1 && is_beta_op o1' && is_beta_op o2 && Either? (rc_b (get_op_b o1) (get_op_b o2)) then 
+    comm_ind_left_b (sel_b l k) (sel_b a k) (sel_b b k) (get_op_b o1) (get_op_b o2) (get_op_b o1')
+  else comm_ind_left_ne l a b o1 o2 o1'
+
+val comm_ind_lca_a (l:concrete_st_a) (ol o1 o2:op_a)
+  : Lemma (requires Either? (rc_a o1 o2) /\
+                    eq_a (merge_a l (do_a l o1) (do_a l o2)) (do_a (do_a l o2) o1))
+          (ensures eq_a (merge_a (do_a l ol) (do_a (do_a l ol) o1) (do_a (do_a l ol) o2)) (do_a (do_a (do_a l ol) o2) o1))
+
+val comm_ind_lca_b (l:concrete_st_b) (ol o1 o2:op_b)
+  : Lemma (requires Either? (rc_b o1 o2) /\
+                    eq_b (merge_b l (do_b l o1) (do_b l o2)) (do_b (do_b l o2) o1))
+          (ensures eq_b (merge_b (do_b l ol) (do_b (do_b l ol) o1) (do_b (do_b l ol) o2)) (do_b (do_b (do_b l ol) o2) o1))
+          
+val comm_ind_lca_ne (l:concrete_st) (ol o1 o2:op_t)
+  : Lemma (requires Either? (rc o1 o2) /\ 
+                    ~ (get_key ol = get_key o1 /\ get_key ol = get_key o2 /\
+                       (is_alpha_op ol /\ is_alpha_op o1 /\ is_alpha_op o2) /\
+                       (is_beta_op ol /\ is_beta_op o1 /\ is_beta_op o2)) /\
+                    eq (merge l (do l o1) (do l o2)) (do (do l o2) o1))
+          (ensures eq (merge (do l ol) (do (do l ol) o1) (do (do l ol) o2)) (do (do (do l ol) o2) o1)) 
+          
+let comm_ind_lca (l:concrete_st) (ol o1 o2:op_t)
+  : Lemma (requires Either? (rc o1 o2) /\
+                    distinct_ops o1 o2 /\ distinct_ops o1 ol /\ distinct_ops o2 ol /\
+                    eq (merge l (do l o1) (do l o2)) (do (do l o2) o1))
+          (ensures eq (merge (do l ol) (do (do l ol) o1) (do (do l ol) o2)) (do (do (do l ol) o2) o1)) =
+  let k = get_key ol in
+  if get_key ol = get_key o1 && get_key ol = get_key o2 && is_alpha_op ol && is_alpha_op o1 && is_alpha_op o2 then
+    comm_ind_lca_a (sel_a l k) (get_op_a ol) (get_op_a o1) (get_op_a o2)
+  else if get_key ol = get_key o1 && get_key ol = get_key o2 && is_beta_op ol && is_beta_op o1 && is_beta_op o2 then
+    comm_ind_lca_b (sel_b l k) (get_op_b ol) (get_op_b o1) (get_op_b o2)
+  else comm_ind_lca_ne l ol o1 o2
+
+val comm_base (o1 o2:op_t) (t:key_t)
+  : Lemma (requires Either? (rc o1 o2) /\ distinct_ops o1 o2)
+          (ensures eq (merge (init_st t) (do (init_st t) o1) (do (init_st t) o2)) (do (do (init_st t) o1) o2))
+
+val comm_inter_base_right_a (l a b c:concrete_st_a) (o1 o2 ob ol:op_a) 
+  : Lemma (requires Either? (rc_a o1 o2) /\ Fst_then_snd? (rc_a ob ol) /\ 
+                    distinct_ops o1 o2 /\ distinct_ops o1 ob /\ distinct_ops o1 ol /\ distinct_ops o2 ob /\ distinct_ops o2 ol /\ distinct_ops ob ol /\
+                    eq_a (merge_a (do_a l ol) (do_a (do_a a ol) o1) (do_a (do_a b ol) o2)) (do_a (do_a (do_a c ol) o1) o2) /\ 
+                    eq_a (merge_a l (do_a a o1) (do_a b o2)) (do_a (do_a c o1) o2) /\
+                    eq_a (merge_a l (do_a a o1) (do_a (do_a b ob) o2)) (do_a (do_a (merge_a l a (do_a b ob)) o1) o2) /\ //comes from comm_ind_right
+                    eq_a (merge_a (do_a l ol) (do_a a ol) (do_a (do_a b ob) ol)) (do_a (do_a c ob) ol)) //comes from intermediate_base_zero_op
+          (ensures eq_a (merge_a (do_a l ol) (do_a (do_a a ol) o1) (do_a (do_a (do_a b ob) ol) o2)) (do_a (do_a (do_a (do_a c ob) ol) o1) o2))
+
+val comm_inter_base_right_b (l a b c:concrete_st_b) (o1 o2 ob ol:op_b) 
+  : Lemma (requires Either? (rc_b o1 o2) /\ Fst_then_snd? (rc_b ob ol) /\ 
+                    distinct_ops o1 o2 /\ distinct_ops o1 ob /\ distinct_ops o1 ol /\ distinct_ops o2 ob /\ distinct_ops o2 ol /\ distinct_ops ob ol /\
+                    eq_b (merge_b (do_b l ol) (do_b (do_b a ol) o1) (do_b (do_b b ol) o2)) (do_b (do_b (do_b c ol) o1) o2) /\ 
+                    eq_b (merge_b l (do_b a o1) (do_b b o2)) (do_b (do_b c o1) o2) /\
+                    eq_b (merge_b l (do_b a o1) (do_b (do_b b ob) o2)) (do_b (do_b (merge_b l a (do_b b ob)) o1) o2) /\ //comes from comm_ind_right
+                    eq_b (merge_b (do_b l ol) (do_b a ol) (do_b (do_b b ob) ol)) (do_b (do_b c ob) ol)) //comes from intermediate_base_zero_op
+          (ensures eq_b (merge_b (do_b l ol) (do_b (do_b a ol) o1) (do_b (do_b (do_b b ob) ol) o2)) (do_b (do_b (do_b (do_b c ob) ol) o1) o2))
+
+val comm_inter_base_right_ne (l a b c:concrete_st) (o1 o2 ob ol:op_t) 
+  : Lemma (requires Either? (rc o1 o2) /\ Fst_then_snd? (rc ob ol) /\ 
+                    distinct_ops o1 o2 /\ distinct_ops o1 ob /\ distinct_ops o1 ol /\ distinct_ops o2 ob /\ distinct_ops o2 ol /\ distinct_ops ob ol /\
+                    ~ (get_key ol = get_key ob && get_key o1 = get_key ob && get_key o2 = get_key ob /\
+                       (is_alpha_op o1 /\ is_alpha_op o2 /\ is_alpha_op ob /\ is_alpha_op ol) /\
+                       (is_beta_op o1 /\ is_beta_op o2 /\ is_beta_op ob /\ is_beta_op ol)) /\
+                    eq (merge (do l ol) (do (do a ol) o1) (do (do b ol) o2)) (do (do (do c ol) o1) o2) /\ 
+                    eq (merge l (do a o1) (do b o2)) (do (do c o1) o2) /\
+                    eq (merge l (do a o1) (do (do b ob) o2)) (do (do (merge l a (do b ob)) o1) o2) /\ //comes from comm_ind_right
+                    eq (merge (do l ol) (do a ol) (do (do b ob) ol)) (do (do c ob) ol)) //comes from intermediate_base_zero_op
+          (ensures eq (merge (do l ol) (do (do a ol) o1) (do (do (do b ob) ol) o2)) (do (do (do (do c ob) ol) o1) o2)) 
+          
+let comm_inter_base_right (l a b c:concrete_st) (o1 o2 ob ol:op_t) 
+  : Lemma (requires Either? (rc o1 o2) /\ Fst_then_snd? (rc ob ol) /\ 
+                    distinct_ops o1 o2 /\ distinct_ops o1 ob /\ distinct_ops o1 ol /\ distinct_ops o2 ob /\ distinct_ops o2 ol /\ distinct_ops ob ol /\
+                    eq (merge (do l ol) (do (do a ol) o1) (do (do b ol) o2)) (do (do (do c ol) o1) o2) /\ 
+                    eq (merge l (do a o1) (do b o2)) (do (do c o1) o2) /\
+                    eq (merge l (do a o1) (do (do b ob) o2)) (do (do (merge l a (do b ob)) o1) o2) /\ //comes from comm_ind_right
+                    eq (merge (do l ol) (do a ol) (do (do b ob) ol)) (do (do c ob) ol)) //comes from intermediate_base_zero_op
+          (ensures eq (merge (do l ol) (do (do a ol) o1) (do (do (do b ob) ol) o2)) (do (do (do (do c ob) ol) o1) o2)) =
+  let k = get_key ob in
+  if get_key ol = k && get_key o1 = k && get_key o2 = k && is_alpha_op o1 && is_alpha_op o2 && is_alpha_op ob && is_alpha_op ol && Either? (rc_a (get_op_a o1) (get_op_a o2)) && Fst_then_snd? (rc_a (get_op_a ob) (get_op_a ol)) then
+    comm_inter_base_right_a (sel_a l k) (sel_a a k) (sel_a b k) (sel_a c k) (get_op_a o1) (get_op_a o2) (get_op_a ob) (get_op_a ol)
+  else if get_key ol = k && get_key o1 = k && get_key o2 = k && is_beta_op o1 && is_beta_op o2 && is_beta_op ob && is_beta_op ol && Either? (rc_b (get_op_b o1) (get_op_b o2)) && Fst_then_snd? (rc_b (get_op_b ob) (get_op_b ol)) then
+    comm_inter_base_right_b (sel_b l k) (sel_b a k) (sel_b b k) (sel_b c k) (get_op_b o1) (get_op_b o2) (get_op_b ob) (get_op_b ol)
+  else comm_inter_base_right_ne l a b c o1 o2 ob ol
+
+val comm_inter_base_left_a (l a b c:concrete_st_a) (o1 o2 ob ol:op_a) 
+  : Lemma (requires Either? (rc_a o1 o2) /\ Fst_then_snd? (rc_a ob ol) /\ 
+                    distinct_ops o1 o2 /\ distinct_ops o1 ob /\ distinct_ops o1 ol /\ distinct_ops o2 ob /\ distinct_ops o2 ol /\ distinct_ops ob ol /\
+                    eq_a (merge_a (do_a l ol) (do_a (do_a a ol) o1) (do_a (do_a b ol) o2)) (do_a (do_a (do_a c ol) o1) o2) /\ 
+                    eq_a (merge_a l (do_a a o1) (do_a b o2)) (do_a (do_a c o1) o2) /\
+                    eq_a (merge_a l (do_a a o1) (do_a (do_a b ob) o2)) (do_a (do_a (merge_a l a (do_a b ob)) o1) o2) /\ //comes from comm_ind_left
+                    eq_a (merge_a (do_a l ol) (do_a (do_a a ob) ol) (do_a b ol)) (do_a (do_a c ob) ol)) //comes from intermediate_base_zero_op
+          (ensures eq_a (merge_a (do_a l ol) (do_a (do_a (do_a a ob) ol) o1) (do_a (do_a b ol) o2)) (do_a (do_a (do_a (do_a c ob) ol) o1) o2))
+
+val comm_inter_base_left_b (l a b c:concrete_st_b) (o1 o2 ob ol:op_b) 
+  : Lemma (requires Either? (rc_b o1 o2) /\ Fst_then_snd? (rc_b ob ol) /\ 
+                    distinct_ops o1 o2 /\ distinct_ops o1 ob /\ distinct_ops o1 ol /\ distinct_ops o2 ob /\ distinct_ops o2 ol /\ distinct_ops ob ol /\
+                    eq_b (merge_b (do_b l ol) (do_b (do_b a ol) o1) (do_b (do_b b ol) o2)) (do_b (do_b (do_b c ol) o1) o2) /\ 
+                    eq_b (merge_b l (do_b a o1) (do_b b o2)) (do_b (do_b c o1) o2) /\
+                    eq_b (merge_b l (do_b a o1) (do_b (do_b b ob) o2)) (do_b (do_b (merge_b l a (do_b b ob)) o1) o2) /\ //comes from comm_ind_left
+                    eq_b (merge_b (do_b l ol) (do_b (do_b a ob) ol) (do_b b ol)) (do_b (do_b c ob) ol)) //comes from intermediate_base_zero_op
+          (ensures eq_b (merge_b (do_b l ol) (do_b (do_b (do_b a ob) ol) o1) (do_b (do_b b ol) o2)) (do_b (do_b (do_b (do_b c ob) ol) o1) o2))
+
+val comm_inter_base_left_ne (l a b c:concrete_st) (o1 o2 ob ol:op_t) 
+  : Lemma (requires Either? (rc o1 o2) /\ Fst_then_snd? (rc ob ol) /\ 
+                    distinct_ops o1 o2 /\ distinct_ops o1 ob /\ distinct_ops o1 ol /\ distinct_ops o2 ob /\ distinct_ops o2 ol /\ distinct_ops ob ol /\
+                    ~ (get_key ol = get_key ob && get_key o1 = get_key ob && get_key o2 = get_key ob /\
+                       (is_alpha_op o1 /\ is_alpha_op o2 /\ is_alpha_op ob /\ is_alpha_op ol) /\
+                       (is_beta_op o1 /\ is_beta_op o2 /\ is_beta_op ob /\ is_beta_op ol)) /\
+                    eq (merge (do l ol) (do (do a ol) o1) (do (do b ol) o2)) (do (do (do c ol) o1) o2) /\ 
+                    eq (merge l (do a o1) (do b o2)) (do (do c o1) o2) /\
+                    eq (merge l (do a o1) (do (do b ob) o2)) (do (do (merge l a (do b ob)) o1) o2) /\ //comes from comm_ind_left
+                    eq (merge (do l ol) (do (do a ob) ol) (do b ol)) (do (do c ob) ol)) //comes from intermediate_base_zero_op
+          (ensures eq (merge (do l ol) (do (do (do a ob) ol) o1) (do (do b ol) o2)) (do (do (do (do c ob) ol) o1) o2))
+          
+let comm_inter_base_left (l a b c:concrete_st) (o1 o2 ob ol:op_t) 
+  : Lemma (requires Either? (rc o1 o2) /\ Fst_then_snd? (rc ob ol) /\ 
+                    distinct_ops o1 o2 /\ distinct_ops o1 ob /\ distinct_ops o1 ol /\ distinct_ops o2 ob /\ distinct_ops o2 ol /\ distinct_ops ob ol /\
+                    eq (merge (do l ol) (do (do a ol) o1) (do (do b ol) o2)) (do (do (do c ol) o1) o2) /\ 
+                    eq (merge l (do a o1) (do b o2)) (do (do c o1) o2) /\
+                    eq (merge l (do a o1) (do (do b ob) o2)) (do (do (merge l a (do b ob)) o1) o2) /\ //comes from comm_ind_left
+                    eq (merge (do l ol) (do (do a ob) ol) (do b ol)) (do (do c ob) ol)) //comes from intermediate_base_zero_op
+          (ensures eq (merge (do l ol) (do (do (do a ob) ol) o1) (do (do b ol) o2)) (do (do (do (do c ob) ol) o1) o2)) =
+  let k = get_key ob in
+  if get_key ol = k && get_key o1 = k && get_key o2 = k && is_alpha_op o1 && is_alpha_op o2 && is_alpha_op ob && is_alpha_op ol && Either? (rc_a (get_op_a o1) (get_op_a o2)) && Fst_then_snd? (rc_a (get_op_a ob) (get_op_a ol)) then
+    comm_inter_base_left_a (sel_a l k) (sel_a a k) (sel_a b k) (sel_a c k) (get_op_a o1) (get_op_a o2) (get_op_a ob) (get_op_a ol)
+  else if get_key ol = k && get_key o1 = k && get_key o2 = k && is_beta_op o1 && is_beta_op o2 && is_beta_op ob && is_beta_op ol && Either? (rc_b (get_op_b o1) (get_op_b o2)) && Fst_then_snd? (rc_b (get_op_b ob) (get_op_b ol)) then
+    comm_inter_base_left_b (sel_b l k) (sel_b a k) (sel_b b k) (sel_b c k) (get_op_b o1) (get_op_b o2) (get_op_b ob) (get_op_b ol)
+  else comm_inter_base_left_ne l a b c o1 o2 ob ol
+
+val comm_inter_right_a (l a b c:concrete_st_a) (o1 o2 ob ol o:op_a)
+  : Lemma (requires Either? (rc_a o1 o2) /\ Fst_then_snd? (rc_a ob ol) /\
+                    distinct_ops o1 o2 /\ distinct_ops o1 ob /\ distinct_ops o1 ol /\ distinct_ops o1 o /\ distinct_ops o2 ob /\ 
+                    distinct_ops o2 ol /\ distinct_ops o2 o /\ distinct_ops ob ol /\ distinct_ops ob o /\ distinct_ops ol o /\
+                    get_rid o <> get_rid ol /\
+                    (~ (Either? (rc_a o ob)) \/ Fst_then_snd? (rc_a o ol)) /\
+                    eq_a (merge_a (do_a l ol) (do_a (do_a a ol) o1) (do_a (do_a (do_a b ob) ol) o2)) (do_a (do_a (do_a (do_a c ob) ol) o1) o2))
+          (ensures eq_a (merge_a (do_a l ol) (do_a (do_a a ol) o1) (do_a (do_a (do_a (do_a b o) ob) ol) o2)) (do_a (do_a (do_a (do_a (do_a c o) ob) ol) o1) o2))
+
+val comm_inter_right_b (l a b c:concrete_st_b) (o1 o2 ob ol o:op_b)
+  : Lemma (requires Either? (rc_b o1 o2) /\ Fst_then_snd? (rc_b ob ol) /\
+                    distinct_ops o1 o2 /\ distinct_ops o1 ob /\ distinct_ops o1 ol /\ distinct_ops o1 o /\ distinct_ops o2 ob /\ 
+                    distinct_ops o2 ol /\ distinct_ops o2 o /\ distinct_ops ob ol /\ distinct_ops ob o /\ distinct_ops ol o /\
+                    get_rid o <> get_rid ol /\
+                    (~ (Either? (rc_b o ob)) \/ Fst_then_snd? (rc_b o ol)) /\
+                    eq_b (merge_b (do_b l ol) (do_b (do_b a ol) o1) (do_b (do_b (do_b b ob) ol) o2)) (do_b (do_b (do_b (do_b c ob) ol) o1) o2))
+          (ensures eq_b (merge_b (do_b l ol) (do_b (do_b a ol) o1) (do_b (do_b (do_b (do_b b o) ob) ol) o2)) (do_b (do_b (do_b (do_b (do_b c o) ob) ol) o1) o2))
+      
+val comm_inter_right_ne (l a b c:concrete_st) (o1 o2 ob ol o:op_t) 
+  : Lemma (requires Either? (rc o1 o2) /\ Fst_then_snd? (rc ob ol) /\ 
+                    distinct_ops o1 o2 /\ distinct_ops o1 ob /\ distinct_ops o1 ol /\ distinct_ops o1 o /\ distinct_ops o2 ob /\ 
+                    distinct_ops o2 ol /\ distinct_ops o2 o /\ distinct_ops ob ol /\ distinct_ops ob o /\ distinct_ops ol o /\
+                    ~ (get_key o2 = get_key o /\ get_key o2 = get_key ob /\
+                       (is_alpha_op o1 /\ is_alpha_op o2 /\ is_alpha_op ob /\ Fst_then_snd? (rc_a (get_op_a o1) (get_op_a o2)) /\ Fst_then_snd? (rc_a (get_op_a ob) (get_op_a ol))) /\
+                       (is_beta_op o1 /\ is_beta_op ob /\ Fst_then_snd? (rc_b (get_op_b o1) (get_op_b o2)) /\ Fst_then_snd? (rc_b (get_op_b ob) (get_op_b ol))) /\
+                       (~ (Either? (rc_a (get_op_a o) (get_op_a ob))) \/ Fst_then_snd? (rc_a (get_op_a o) (get_op_a ol))) /\
+                       (~ (Either? (rc_b (get_op_b o) (get_op_b ob))) \/ Fst_then_snd? (rc_b (get_op_b o) (get_op_b ol)))) /\
+                    get_rid o <> get_rid ol (*o,ol must be concurrent*) /\
+                    (~ (Either? (rc o ob)) \/ Fst_then_snd? (rc o ol)) /\
+                    eq (merge (do l ol) (do (do a ol) o1) (do (do (do b ob) ol) o2)) (do (do (do (do c ob) ol) o1) o2))
+          (ensures eq (merge (do l ol) (do (do a ol) o1) (do (do (do (do b o) ob) ol) o2)) (do (do (do (do (do c o) ob) ol) o1) o2))
+
+let comm_inter_right (l a b c:concrete_st) (o1 o2 ob ol o:op_t)
+  : Lemma (requires Either? (rc o1 o2) /\ Fst_then_snd? (rc ob ol) /\ 
+                    distinct_ops o1 o2 /\ distinct_ops o1 ob /\ distinct_ops o1 ol /\ distinct_ops o1 o /\ distinct_ops o2 ob /\ 
+                    distinct_ops o2 ol /\ distinct_ops o2 o /\ distinct_ops ob ol /\ distinct_ops ob o /\ distinct_ops ol o /\
+                    get_rid o <> get_rid ol (*o,ol must be concurrent*) /\
+                    (~ (Either? (rc o ob)) \/ Fst_then_snd? (rc o ol)) /\
+                    eq (merge (do l ol) (do (do a ol) o1) (do (do (do b ob) ol) o2)) (do (do (do (do c ob) ol) o1) o2))
+          (ensures eq (merge (do l ol) (do (do a ol) o1) (do (do (do (do b o) ob) ol) o2)) (do (do (do (do (do c o) ob) ol) o1) o2)) =
+  let k = get_key o in
+  if get_key o1 = k && get_key o2 = k && get_key ob = k && get_key ol = k && is_alpha_op o1 && is_alpha_op o2 && is_alpha_op ob && is_alpha_op ol && is_alpha_op o && Fst_then_snd? (rc_a (get_op_a o1) (get_op_a o2)) && Fst_then_snd? (rc_a (get_op_a ob) (get_op_a ol)) && (Fst_then_snd? (rc_a (get_op_a o) (get_op_a ob)) || Snd_then_fst? (rc_a (get_op_a o) (get_op_a ob)) || Fst_then_snd? (rc_a (get_op_a o) (get_op_a ol))) then 
+    comm_inter_right_a (sel_a l k) (sel_a a k) (sel_a b k) (sel_a c k) (get_op_a o1) (get_op_a o2) (get_op_a ob) (get_op_a ol) (get_op_a o)
+  else if get_key o1 = k && get_key o2 = k && get_key ob = k && get_key ol = k && is_beta_op o1 && is_beta_op o2 && is_beta_op ob && is_beta_op ol && is_beta_op o && Fst_then_snd? (rc_b (get_op_b o1) (get_op_b o2)) && Fst_then_snd? (rc_b (get_op_b ob) (get_op_b ol)) && (Fst_then_snd? (rc_b (get_op_b o) (get_op_b ob)) || Snd_then_fst? (rc_b (get_op_b o) (get_op_b ob)) || Fst_then_snd? (rc_b (get_op_b o) (get_op_b ol))) then
+    comm_inter_right_b (sel_b l k) (sel_b a k) (sel_b b k) (sel_b c k) (get_op_b o1) (get_op_b o2) (get_op_b ob) (get_op_b ol) (get_op_b o)
+  else comm_inter_right_ne l a b c o1 o2 ob ol o
+
+val comm_inter_left_a (l a b c:concrete_st_a) (o1 o2 ob ol o:op_a)
+  : Lemma (requires Either? (rc_a o1 o2) /\ Fst_then_snd? (rc_a ob ol) /\
+                    distinct_ops o1 o2 /\ distinct_ops o1 ob /\ distinct_ops o1 ol /\ distinct_ops o1 o /\ distinct_ops o2 ob /\ 
+                    distinct_ops o2 ol /\ distinct_ops o2 o /\ distinct_ops ob ol /\ distinct_ops ob o /\ distinct_ops ol o /\
+                    get_rid o <> get_rid ol /\
+                    (~ (Either? (rc_a o ob)) \/ Fst_then_snd? (rc_a o ol)) /\
+                    eq_a (merge_a (do_a l ol) (do_a (do_a (do_a a ob) ol) o1) (do_a (do_a b ol) o2)) (do_a (do_a (do_a (do_a c ob) ol) o1) o2))
+          (ensures eq_a (merge_a (do_a l ol) (do_a (do_a (do_a (do_a a o) ob) ol) o1) (do_a (do_a b ol) o2)) (do_a (do_a (do_a (do_a (do_a c o) ob) ol) o1) o2))
+
+val comm_inter_left_b (l a b c:concrete_st_b) (o1 o2 ob ol o:op_b)
+  : Lemma (requires Either? (rc_b o1 o2) /\ Fst_then_snd? (rc_b ob ol) /\
+                    distinct_ops o1 o2 /\ distinct_ops o1 ob /\ distinct_ops o1 ol /\ distinct_ops o1 o /\ distinct_ops o2 ob /\ 
+                    distinct_ops o2 ol /\ distinct_ops o2 o /\ distinct_ops ob ol /\ distinct_ops ob o /\ distinct_ops ol o /\
+                    get_rid o <> get_rid ol /\
+                    (~ (Either? (rc_b o ob)) \/ Fst_then_snd? (rc_b o ol)) /\
+                    eq_b (merge_b (do_b l ol) (do_b (do_b (do_b a ob) ol) o1) (do_b (do_b b ol) o2)) (do_b (do_b (do_b (do_b c ob) ol) o1) o2))
+          (ensures eq_b (merge_b (do_b l ol) (do_b (do_b (do_b (do_b a o) ob) ol) o1) (do_b (do_b b ol) o2)) (do_b (do_b (do_b (do_b (do_b c o) ob) ol) o1) o2))
+      
+val comm_inter_left_ne (l a b c:concrete_st) (o1 o2 ob ol o:op_t) 
+  : Lemma (requires Either? (rc o1 o2) /\ Fst_then_snd? (rc ob ol) /\ 
+                    distinct_ops o1 o2 /\ distinct_ops o1 ob /\ distinct_ops o1 ol /\ distinct_ops o1 o /\ distinct_ops o2 ob /\ 
+                    distinct_ops o2 ol /\ distinct_ops o2 o /\ distinct_ops ob ol /\ distinct_ops ob o /\ distinct_ops ol o /\
+                    ~ (get_key o2 = get_key o /\ get_key o2 = get_key ob /\
+                       (is_alpha_op o1 /\ is_alpha_op o2 /\ is_alpha_op ob /\ Fst_then_snd? (rc_a (get_op_a o1) (get_op_a o2)) /\ Fst_then_snd? (rc_a (get_op_a ob) (get_op_a ol))) /\
+                       (is_beta_op o1 /\ is_beta_op ob /\ Fst_then_snd? (rc_b (get_op_b o1) (get_op_b o2)) /\ Fst_then_snd? (rc_b (get_op_b ob) (get_op_b ol))) /\
+                       (~ (Either? (rc_a (get_op_a o) (get_op_a ob))) \/ Fst_then_snd? (rc_a (get_op_a o) (get_op_a ol))) /\
+                       (~ (Either? (rc_b (get_op_b o) (get_op_b ob))) \/ Fst_then_snd? (rc_b (get_op_b o) (get_op_b ol)))) /\
+                    get_rid o <> get_rid ol (*o,ol must be concurrent*) /\
+                    (~ (Either? (rc o ob)) \/ Fst_then_snd? (rc o ol)) /\
+                    eq (merge (do l ol) (do (do (do a ob) ol) o1) (do (do b ol) o2)) (do (do (do (do c ob) ol) o1) o2))
+          (ensures eq (merge (do l ol) (do (do (do (do a o) ob) ol) o1) (do (do b ol) o2)) (do (do (do (do (do c o) ob) ol) o1) o2))
+
+let comm_inter_left (l a b c:concrete_st) (o1 o2 ob ol o:op_t)
+  : Lemma (requires Either? (rc o1 o2) /\ Fst_then_snd? (rc ob ol) /\ 
+                    distinct_ops o1 o2 /\ distinct_ops o1 ob /\ distinct_ops o1 ol /\ distinct_ops o1 o /\ distinct_ops o2 ob /\ 
+                    distinct_ops o2 ol /\ distinct_ops o2 o /\ distinct_ops ob ol /\ distinct_ops ob o /\ distinct_ops ol o /\
+                    get_rid o <> get_rid ol (*o,ol must be concurrent*) /\
+                    (~ (Either? (rc o ob)) \/ Fst_then_snd? (rc o ol)) /\
+                    eq (merge (do l ol) (do (do (do a ob) ol) o1) (do (do b ol) o2)) (do (do (do (do c ob) ol) o1) o2))
+          (ensures eq (merge (do l ol) (do (do (do (do a o) ob) ol) o1) (do (do b ol) o2)) (do (do (do (do (do c o) ob) ol) o1) o2)) =
+  let k = get_key o in
+  if get_key o1 = k && get_key o2 = k && get_key ob = k && get_key ol = k && is_alpha_op o1 && is_alpha_op o2 && is_alpha_op ob && is_alpha_op ol && is_alpha_op o && Fst_then_snd? (rc_a (get_op_a o1) (get_op_a o2)) && Fst_then_snd? (rc_a (get_op_a ob) (get_op_a ol)) && (Fst_then_snd? (rc_a (get_op_a o) (get_op_a ob)) || Snd_then_fst? (rc_a (get_op_a o) (get_op_a ob)) || Fst_then_snd? (rc_a (get_op_a o) (get_op_a ol))) then 
+    comm_inter_left_a (sel_a l k) (sel_a a k) (sel_a b k) (sel_a c k) (get_op_a o1) (get_op_a o2) (get_op_a ob) (get_op_a ol) (get_op_a o)
+  else if get_key o1 = k && get_key o2 = k && get_key ob = k && get_key ol = k && is_beta_op o1 && is_beta_op o2 && is_beta_op ob && is_beta_op ol && is_beta_op o && Fst_then_snd? (rc_b (get_op_b o1) (get_op_b o2)) && Fst_then_snd? (rc_b (get_op_b ob) (get_op_b ol)) && (Fst_then_snd? (rc_b (get_op_b o) (get_op_b ob)) || Snd_then_fst? (rc_b (get_op_b o) (get_op_b ob)) || Fst_then_snd? (rc_b (get_op_b o) (get_op_b ol))) then
+    comm_inter_left_b (sel_b l k) (sel_b a k) (sel_b b k) (sel_b c k) (get_op_b o1) (get_op_b o2) (get_op_b ob) (get_op_b ol) (get_op_b o)
+  else comm_inter_left_ne l a b c o1 o2 ob ol o
+
+val comm_inter_lca_a (l a b c:concrete_st_a) (o1 o2 ol:op_a)
+  : Lemma (requires Either? (rc_a o1 o2) /\ 
+                    distinct_ops o1 o2 /\ distinct_ops o1 ol /\ distinct_ops ol o2 /\
+                    (exists o'. Fst_then_snd? (rc_a o' ol)) /\
+                    eq_a (merge_a l (do_a a o1) (do_a b o2)) (do_a (do_a c o1) o2))
+          (ensures eq_a (merge_a (do_a l ol) (do_a (do_a a ol) o1) (do_a (do_a b ol) o2)) (do_a (do_a (do_a c ol) o1) o2)) 
+
+val comm_inter_lca_b (l a b c:concrete_st_b) (o1 o2 ol:op_b)
+  : Lemma (requires Either? (rc_b o1 o2) /\ 
+                    distinct_ops o1 o2 /\ distinct_ops o1 ol /\ distinct_ops ol o2 /\
+                    (exists o'. Fst_then_snd? (rc_b o' ol)) /\
+                    eq_b (merge_b l (do_b a o1) (do_b b o2)) (do_b (do_b c o1) o2))
+          (ensures eq_b (merge_b (do_b l ol) (do_b (do_b a ol) o1) (do_b (do_b b ol) o2)) (do_b (do_b (do_b c ol) o1) o2)) 
+
+val comm_inter_lca_ne (l a b c:concrete_st) (o1 o2 ol:op_t)
+  : Lemma (requires Either? (rc o1 o2) /\ 
+                    distinct_ops o1 o2 /\ distinct_ops o1 ol /\ distinct_ops ol o2 /\
+                    ~ (get_key ol = get_key o1 /\ get_key ol = get_key o2 /\
+                       (is_alpha_op o1 /\ is_alpha_op o2 /\ is_alpha_op ol) /\
+                       (is_beta_op o1 /\ is_beta_op o2 /\ is_beta_op ol)) /\
+                    (exists o'. Fst_then_snd? (rc o' ol)) /\
+                    eq (merge l (do a o1) (do b o2)) (do (do c o1) o2))
+          (ensures eq (merge (do l ol) (do (do a ol) o1) (do (do b ol) o2)) (do (do (do c ol) o1) o2))
+
+let comm_inter_lca (l a b c:concrete_st) (o1 o2 ol:op_t)
+  : Lemma (requires Either? (rc o1 o2) /\ 
+                    distinct_ops o1 o2 /\ distinct_ops o1 ol /\ distinct_ops ol o2 /\
+                    (exists o'. Fst_then_snd? (rc o' ol)) /\
+                    eq (merge l (do a o1) (do b o2)) (do (do c o1) o2))
+          (ensures eq (merge (do l ol) (do (do a ol) o1) (do (do b ol) o2)) (do (do (do c ol) o1) o2)) =
+  let k = get_key ol in
+  if get_key o1 = k && get_key o2 = k && is_alpha_op o1 && is_alpha_op o2 && is_alpha_op ol then
+    comm_inter_lca_a (sel_a l k) (sel_a a k) (sel_a b k) (sel_a c k) (get_op_a o1) (get_op_a o2) (get_op_a ol)
+  else if get_key o1 = k && get_key o2 = k && is_beta_op o1 && is_beta_op o2 && is_beta_op ol then
+    comm_inter_lca_b (sel_b l k) (sel_b a k) (sel_b b k) (sel_b c k) (get_op_b o1) (get_op_b o2) (get_op_b ol) 
+  else comm_inter_lca_ne l a b c o1 o2 ol
 
 
 
